WIP

code/Yazi.Tree.fst
@@ -16,53 +16,106 @@ open Spec.Tree
 open Yazi.Deflate.Constants
 open Yazi.Tree.Types
 
+type cmp_impl (spec: SH.cmp_spec) =
+    tl: tree_len_t
+  -> tree: B.lbuffer ct_data (Ghost.reveal tl)
+  -> depth: tree_depth_t
+  -> n: U32.t
+  -> m: U32.t
+  -> ST.Stack bool
+  (requires fun h ->
+    U32.v n < tl /\ U32.v m < tl /\ B.live h tree /\ B.live h depth)
+  (ensures fun h0 res h1 ->
+    B.modifies B.loc_none h0 h1 /\
+    (res == true <==> spec tl (B.as_seq h1 tree) (B.as_seq h1 depth) n m))
+
+val build_cmp: tl: tree_len_t
+  -> tree: B.lbuffer ct_data (Ghost.reveal tl)
+  -> depth: tree_depth_t
+  -> n: U32.t
+  -> m: U32.t
+  -> ST.Stack bool
+  (requires fun h ->
+    U32.v n < tl /\ U32.v m < tl /\ B.live h tree /\ B.live h depth)
+  (ensures fun h0 res h1 ->
+    B.modifies B.loc_none h0 h1 /\
+    (res == true <==> SH.build_cmp tl (B.as_seq h1 tree) (B.as_seq h1 depth) n m))
+let build_cmp = fun tl tree depth n m ->
+  ST.push_frame ();
+  let nfd = (tree.(n)).freq_or_code in
+  let mfd = (tree.(m)).freq_or_code in
+  let res = if nfd `U16.lt` mfd then
+    true
+  else if nfd `U16.eq` mfd then
+    let dn = depth.(n) in
+    let dm = depth.(m) in
+    if dn `U8.lt` dm then
+      true
+    else if dn `U8.eq` dm then
+      n `U32.lte` m
+    else
+      false
+  else
+    false
+  in
+  ST.pop_frame ();
+  res
+
 let htd_seperate
   (h: HS.mem) (heap: tree_heap_t)
   (tree: B.buffer ct_data) (depth: tree_depth_t) =
   B.live h heap /\ B.live h tree /\ B.live h depth /\
   B.disjoint heap tree /\ B.disjoint heap depth /\ B.disjoint tree depth
 
-inline_for_extraction
-let smaller
-  (tl: tree_len_t) (tree: B.lbuffer ct_data (Ghost.reveal tl))
-  (depth: tree_depth_t) (n m: U32.t):
-  ST.Stack bool
-  (requires fun h ->
-    U32.v n < tl /\ U32.v m < tl /\
-    B.live h tree /\ B.live h depth)
-  (ensures fun h0 res h1 ->
-    B.modifies B.loc_none h0 h1 /\
-    (res <==> SH.smaller h1 tl tree depth n m)) =
-  let nfd = (tree.(n)).freq_or_code in
-  let mfd = (tree.(m)).freq_or_code in
-  if nfd `U16.lt` mfd then
-    true
-  else if nfd `U16.eq` mfd then
-    let dn = depth.(n) in
-    let dm = depth.(m) in
-    dn `U8.lte` dm
-  else
-    false
-
 let heap_common_pre_cond
-  (h: HS.mem) (heap: tree_heap_t) (hl: heap_len_t)
+  (cmp: SH.cmp_spec) (h: HS.mem)
+  (heap: tree_heap_t) (hl: heap_len_t)
   (tl: tree_len_t) (tree: B.lbuffer ct_data tl)
   (depth: tree_depth_t)
   (i: U32.t{U32.v i < tl})
   (root: Ghost.erased (heap_internal_index_t hl))
   (hole: heap_index_t hl) =
   let open U32 in
-  let partial_well_formed = SH.partial_well_formed h heap hl tl tree depth in
-  v root <= v hole /\
+  let partial_well_formed = SH.partial_well_formed cmp h heap hl tl tree depth in
   htd_seperate h heap tree depth /\
-  SH.smaller h tl tree depth (B.as_seq h heap).[v hole] i /\
+  (let heap = B.as_seq h heap in
+  v heap.[v hole] < tl /\ v heap.[v hole] < B.length depth /\
+  cmp tl (B.as_seq h tree) (B.as_seq h depth) heap.[v hole] i /\
+  v root <= v hole /\
   (v root == v hole ==>
-    partial_well_formed (root +^ 1ul) /\
-    (B.as_seq h heap).[v root] == i) /\
-  (v root < v hole ==> partial_well_formed root)
+    partial_well_formed (root +^ 1ul) /\ heap.[v root] == i) /\
+  (v root < v hole ==> partial_well_formed root))
+
+unfold let heap_smallest_post_cond
+  (cmp: SH.cmp_spec) (h0: HS.mem) (res: U32.t) (h1: HS.mem)
+  (heap: tree_heap_t) (hl: heap_len_t)
+  (tl: tree_len_t) (tree: B.lbuffer ct_data tl)
+  (depth: tree_depth_t)
+  (i: U32.t{U32.v i < tl})
+  (root: Ghost.erased (heap_internal_index_t hl))
+  (hole: heap_internal_index_t hl) =
+  let open U32 in
+  let heap_elem = SH.heap_elem tl depth in
+  let heap = B.as_seq h1 heap in let hl = v hl in
+  let root = v root in let hole = v hole in let res = v res in
+  let smaller = cmp tl (B.as_seq h0 tree) (B.as_seq h0 depth) in
+  B.modifies B.loc_none h0 h1 /\
+  res <= hl /\ (res == 0 \/ res == hole * 2 \/ res == hole * 2 + 1) /\
+  (res <> 0 ==> heap_elem heap.[res]) /\
+  (let k = if res = 0 then i else heap.[res] in
+  heap_elem heap.[hole] /\
+  heap_elem heap.[hole * 2] /\
+  k `smaller` i /\
+  k `smaller` heap.[hole * 2] /\
+  (hole * 2 + 1 <= hl ==>
+    heap_elem heap.[hole * 2 + 1] /\
+    k `smaller` heap.[hole * 2 + 1]) /\
+  (root == hole ==> k `smaller` heap.[hole]) /\
+  (root < hole ==> heap.[hole] `smaller` k))
 
 inline_for_extraction
 let smallest
+  (#cs: Ghost.erased SH.cmp_spec) (cmp: cmp_impl cs)
   (heap: tree_heap_t) (hl: heap_len_t)
   (tl: tree_len_t) (tree: B.lbuffer ct_data tl)
   (depth: tree_depth_t)
@@ -70,39 +123,28 @@ let smallest
   (root: Ghost.erased (heap_internal_index_t hl))
   (hole: heap_internal_index_t hl):
   ST.Stack U32.t
-  (requires fun h -> heap_common_pre_cond h heap hl tl tree depth i root hole)
+  (requires fun h -> heap_common_pre_cond cs h heap hl tl tree depth i root hole)
   (ensures fun h0 res h1 ->
-    let heap = B.as_seq h1 heap in let hl = U32.v hl in
-    let root = U32.v root in let hole = U32.v hole in
-    let res = U32.v res in
-    let smaller' = SH.smaller h1 tl tree depth in
-    
-    B.modifies B.loc_none h0 h1 /\
-    res <= hl /\ (res == 0 \/ res == hole * 2 \/ res == hole * 2 + 1) /\
-    (let k = if res = 0 then i else heap.[res] in
-    k `smaller'` i /\
-    k `smaller'` heap.[hole * 2] /\
-    (hole * 2 + 1 <= hl ==> k `smaller'` heap.[hole * 2 + 1]) /\
-    (root == hole ==> k `smaller'` heap.[hole]) /\
-    (root < hole ==> heap.[hole] `smaller'` k))) =
+    heap_smallest_post_cond cs h0 res h1 heap hl tl tree depth i root hole) =
   let open U32 in
   let l = hole *^ 2ul in
   let r = l +^ 1ul in
   let le = heap.(l) in
-  let smaller' = smaller tl tree depth in
-  let h = ST.get () in
+  [@inline_let]
+  let smaller = cmp tl tree depth in
   if r >^ hl then
-    if i `smaller'` le then 0ul else l
+    if i `smaller` le then 0ul else l
   else
     let re = heap.(r) in
-    if i `smaller'` le then
-      if i `smaller'` re then 0ul else r
+    if i `smaller` le then
+      if i `smaller` re then 0ul else r
     else
-      if le `smaller'` re then l else r
+      if le `smaller` re then l else r
 
-#set-options "--z3refresh --z3rlimit 4096 --fuel 0 --ifuel 0"
+#set-options "--z3refresh --z3rlimit 164 --fuel 0 --ifuel 0"
 inline_for_extraction
 let rec do_pqdownheap
+  (#cs: Ghost.erased SH.cmp_spec) (cmp: cmp_impl cs)
   (h_init: Ghost.erased HS.mem)
   (heap: tree_heap_t) (hl: heap_len_t)
   (tl: tree_len_t) (tree: B.lbuffer ct_data tl) (depth: tree_depth_t)
@@ -112,39 +154,40 @@ let rec do_pqdownheap
   ST.Stack unit
   (requires fun h ->
     (B.as_seq h_init heap).[U32.v root] == i /\
-    heap_common_pre_cond h heap hl tl tree depth i root hole /\
+    heap_common_pre_cond cs h heap hl tl tree depth i root hole /\
     SH.permutation_partial (B.as_seq h_init heap) (B.as_seq h heap) root hole)
   (ensures fun h0 _ h1 ->
     B.modifies (B.loc_buffer heap) h0 h1 /\
-    SH.partial_well_formed h1 heap hl tl tree depth root /\
+    SH.partial_well_formed cs h1 heap hl tl tree depth root /\
     Seq.permutation U32.t (B.as_seq h_init heap) (B.as_seq h1 heap))
   (decreases U32.v hl / 2 - U32.v hole) =
   let open U32 in
   if hole >^ hl /^ 2ul then
     heap.(hole) <- i
   else
-    let s = smallest heap hl tl tree depth i root hole in
+    let s = smallest cmp heap hl tl tree depth i root hole in
     if s = 0ul then
       heap.(hole) <- i
     else begin
       heap.(hole) <- heap.(s);
-      do_pqdownheap h_init heap hl tl tree depth i root s
+      do_pqdownheap cmp h_init heap hl tl tree depth i root s
     end
 
 inline_for_extraction
 let pqdownheap
+  (#cs: Ghost.erased SH.cmp_spec) (cmp: cmp_impl cs)
   (heap: tree_heap_t) (hl: heap_len_t)
   (tl: tree_len_t) (tree: B.lbuffer ct_data tl) (depth: tree_depth_t)
   (i: heap_internal_index_t hl):
   ST.Stack unit
   (requires fun h ->
     htd_seperate h heap tree depth /\
-    SH.partial_well_formed h heap hl tl tree depth (U32.add i 1ul))
+    SH.partial_well_formed cs h heap hl tl tree depth (U32.add i 1ul))
   (ensures fun h0 _ h1 ->
     B.modifies (B.loc_buffer heap) h0 h1 /\
-    SH.partial_well_formed h1 heap hl tl tree depth i /\
+    SH.partial_well_formed cs h1 heap hl tl tree depth i /\
     Seq.permutation U32.t (B.as_seq h0 heap) (B.as_seq h1 heap)) =
-  do_pqdownheap (ST.get ()) heap hl tl tree depth heap.(i) i i
+  do_pqdownheap cmp (ST.get ()) heap hl tl tree depth heap.(i) i i
 
 unfold let init_heap_common_cond
   (h: HS.mem)
@@ -170,13 +213,13 @@ unfold let init_heap_common_cond
   (forall i. (i < j /\ U16.v (tree.[i]).freq_or_code > 0) ==>
     Seq.count (uint_to_t i) (Seq.slice heap 1 (hl + 1)) == 1) /\
   (forall i. {:pattern (tree.[i]).freq_or_code}
-    (i < j /\ U16.v (tree.[i]).freq_or_code == 0) ==> U16.v (tree.[i]).dad_or_len == 0) /\
+    i < j /\ U16.v (tree.[i]).freq_or_code == 0 ==> U16.v (tree.[i]).dad_or_len == 0) /\
   (forall i. {:pattern (depth.[i])}
-    (i < j /\ U16.v (tree.[i]).freq_or_code > 0) ==> U8.v depth.[i] = 0) /\
-  (forall i. {:pattern (tree.[i]).freq_or_code}
-    (max_code < i /\ i < j) ==> U16.v (tree.[i]).dad_or_len == 0)
+    i < j /\ U16.v (tree.[i]).freq_or_code > 0 ==> U8.v depth.[i] = 0) /\
+  (forall i. {:pattern (tree.[i]).dad_or_len}
+    max_code < i /\ i < j ==> U16.v (tree.[i]).dad_or_len == 0)
 
-#set-options "--z3refresh --z3rlimit 4096 --fuel 1 --ifuel 1"
+#set-options "--z3refresh --z3rlimit 256 --fuel 1 --ifuel 1"
 [@ CInline ]
 let rec init_heap
   (heap: tree_heap_t) (hl: U32.t{U32.v hl < U32.v heap_size})
@@ -232,7 +275,7 @@ let rec init_heap
       (hl +^ 1ul, j)
   end
 
-#set-options "--z3refresh --z3rlimit 256 --fuel 0 --ifuel 0"
+#set-options "--z3refresh --fuel 0 --ifuel 0"
 [@ CInline ]
 let rec sort_leaves
   (heap: tree_heap_t) (hl: heap_len_t)
@@ -241,13 +284,13 @@ let rec sort_leaves
   ST.Stack unit
   (requires fun h ->
     htd_seperate h heap tree depth /\
-    SH.partial_well_formed h heap hl tl tree depth (U32.add i 1ul))
+    SH.partial_well_formed SH.build_cmp h heap hl tl tree depth (U32.add i 1ul))
   (ensures fun h0 _ h1 ->
     B.modifies (B.loc_buffer heap) h0 h1 /\
-    SH.well_formed h1 heap hl tl tree depth /\
+    SH.well_formed SH.build_cmp h1 heap hl tl tree depth /\
     Seq.permutation U32.t (B.as_seq h0 heap) (B.as_seq h1 heap)) =
   let open U32 in
-  pqdownheap heap hl tl tree depth i;
+  pqdownheap #SH.build_cmp build_cmp heap hl tl tree depth i;
   if i >^ 1ul then
     sort_leaves heap hl tl tree depth (i -^ 1ul)
   else
@@ -262,14 +305,6 @@ let encoder_seperate
   B.disjoint opt_len static_len /\
   B.disjoint opt_len heap /\ B.disjoint opt_len tree /\ B.disjoint opt_len depth /\
   B.disjoint static_len heap /\ B.disjoint static_len tree /\ B.disjoint static_len depth
-
-    // while (s->heap_len < 2) {
-    //     node = s->heap[++(s->heap_len)] = (max_code < 2 ? ++max_code : 0);
-    //     tree[node].Freq = 1;
-    //     s->depth[node] = 0;
-    //     s->opt_len--; if (stree) s->static_len -= stree[node].Len;
-    //     /* node is 0 or 1 so it does not have extra bits */
-    // }
 
 #set-options "--fuel 4 --ifuel 4"
 let build_small_tree
@@ -304,7 +339,7 @@ let build_small_tree
   end else
     let f = (tree.(max_code)).freq_or_code in
     if max_code = 0ul then begin
-      tree.(max_code) <- {
+      tree.(0ul) <- {
         freq_or_code = 0us;
         dad_or_len = 1us
       };
