lib/Lib.Seq.fsti
@@ -59,6 +59,19 @@ let disjoint (#a: eqtype) (s1 s2: Seq.seq a) =
     (Seq.mem x s1 ==> Seq.mem x s2 = false) /\
     (Seq.mem x s2 ==> Seq.mem x s1 = false)
 
+let rec not_mem_forall (#a: eqtype) (v: a) (s: Seq.seq a): Lemma
+  (requires forall i. v <> s.[i])
+  (ensures Seq.mem v s == false)
+  (decreases Seq.length s) =
+  match Seq.length s with
+  | 0 -> ()
+  | _ -> not_mem_forall v (Seq.tail s)
+
+let not_mem_disjoint (#a: eqtype) (v: a) (s: Seq.seq a): Lemma
+  (requires forall i. v <> s.[i])
+  (ensures disjoint (Seq.create 1 v) s) =
+  not_mem_forall v s
+
 let disjoint_comm (#a: eqtype) (s1 s2: Seq.seq a): Lemma
   (requires disjoint s1 s2)
   (ensures disjoint s2 s1)
@@ -97,3 +110,58 @@ let append_empty_seq_r (#a: Type) (s1 s2: Seq.seq a): Lemma
   [SMTPat (Seq.append s1 s2)] =
   Seq.lemma_empty s2;
   Seq.append_empty_r s1
+
+type index_t (#a: eqtype) (s: Seq.seq a) = i:nat{i < Seq.length s}
+
+irreducible let rec index_of (#a: eqtype) (s: Seq.seq a) (v: a{Seq.mem v s}):
+  Tot (i: index_t s{Seq.index s i == v})
+  (decreases Seq.length s) =
+  if Seq.head s = v then 0 else 1 + index_of (Seq.tail s) v
+
+let rec no_dup_index_of (#a: eqtype) (s: Seq.seq a) (v: a{Seq.mem v s}): Lemma
+  (requires no_dup s)
+  (ensures forall i. i <> index_of s v ==> s.[i] <> v)
+  (decreases Seq.length s) =
+  let open Seq in
+  match length s with
+  | 1 -> ()
+  | _ ->
+    let x = create 1 s.[0] in let xs = tail s in
+    assert(equal (x @| xs) s);
+    no_dup_append' x xs;
+    if head s = v then
+      ()
+    else
+      no_dup_index_of (tail s) v
+
+let rec no_dup_index_of_cancel (#a: eqtype) (s: Seq.seq a): Lemma
+  (requires no_dup s)
+  (ensures forall i. index_of s s.[i] == i)
+  (decreases Seq.length s) =
+  let open Seq in
+  match length s with
+  | 0 | 1 -> ()
+  | _ ->
+    let x = create 1 s.[0] in let xs = tail s in
+    assert(equal (x @| xs) s);
+    no_dup_append' x xs;
+    no_dup_index_of_cancel (tail s)
+  
+let rec filter (#a: eqtype) (s: Seq.seq a) (f: a -> bool): Tot (res: Seq.seq a{
+  (forall i. f res.[i] == true /\ Seq.mem res.[i] s) /\
+  (forall i. f s.[i] == true ==> Seq.mem s.[i] res)
+}) (decreases Seq.length s) =
+  let open Seq in
+  if length s = 0 then
+    empty #a
+  else
+    let h = head s in
+    if f h then begin
+      let t = filter (tail s) f in
+      let res = create 1 h @| t in
+      assert(forall i. i > 0 ==> (tail s).[i - 1] == s.[i]);
+      assert(forall i. i > 0 ==> f s.[i] == true ==> mem s.[i] t);
+      lemma_mem_append (create 1 h) t;
+      create 1 h @| t
+    end else
+      filter (tail s) f
