specs/Spec.Heap.fst
@@ -1,7 +1,9 @@
 module Spec.Heap
 
 module B = LowStar.Buffer
+module C = Yazi.Deflate.Constants
 module HS = FStar.HyperStack
+module Math = FStar.Math.Lemmas
 module U16 = FStar.UInt16
 module U32 = FStar.UInt32
 module U8 = FStar.UInt8
@@ -9,39 +11,58 @@ module U8 = FStar.UInt8
 open FStar.Mul
 open FStar.Seq
 open Lib.Seq
+open Yazi.Deflate.Constants
 open Yazi.Tree.Types
 
-let smaller (h: HS.mem)
-  (tl: nat) (tree: B.lbuffer ct_data tl)
-  (depth: tree_depth_t) (i j: U32.t) =
-  let open U32 in
-  let tree = B.as_seq h tree in
-  let depth = B.as_seq h depth in
-  v i < tl /\ v j < tl /\ v i < length depth /\ v j < length depth /\
-  (let fi = U16.v (tree.[v i]).freq_or_code in
-  let fj = U16.v (tree.[v j]).freq_or_code in
-  (fi < fj \/ (fi == fj /\ U8.v depth.[v i] <= U8.v depth.[v j])))
+type cmp_spec =
+    tl: nat 
+  -> tree: Seq.seq ct_data{Seq.length tree == tl}
+  -> depth: Seq.seq U8.t{Seq.length depth == 2 * U32.v C.l_codes + 1}
+  -> i: U32.t{U32.v i < tl /\ U32.v i < length depth}
+  -> j: U32.t{U32.v j < tl /\ U32.v j < length depth}
+  -> Tot bool
 
-let element_in_range (h: HS.mem) (heap: tree_heap_t) (hl: heap_len_t) (tl: nat) =
-  let heap = B.as_seq h heap in
-  (forall (j: pos). {:pattern heap.[j]} j <= U32.v hl ==> U32.v heap.[j] < tl)
+val build_cmp: cmp_spec
+let build_cmp tl tree depth i j =
+  let open U32 in
+  let fi = U16.v (tree.[v i]).freq_or_code in
+  let fj = U16.v (tree.[v j]).freq_or_code in
+  (fi < fj ||
+  (fi = fj && U8.v depth.[v i] < U8.v depth.[v j]) ||
+  (fi = fj && U8.v depth.[v i] = U8.v depth.[v j] && v i <= v j))
+
+let heap_elem (tl: tree_len_t) (depth: tree_depth_t) (a: U32.t) =
+  U32.v a < tl /\ U32.v a < B.length depth
 
 let partial_well_formed
-  (h: HS.mem)
+  (cmp: cmp_spec) (h: HS.mem)
   (heap: tree_heap_t) (hl: heap_len_t)
-  (tl: nat) (tree: B.lbuffer ct_data tl) (depth: tree_depth_t)
+  (tl: tree_len_t) (tree: B.lbuffer ct_data tl) (depth: tree_depth_t)
   (i: heap_index_t hl) =
   let open U32 in
-  let heap' = B.as_seq h heap in
-  element_in_range h heap hl tl /\
-  (forall (k: nat). (v i <= k /\ k <= v hl) ==> (
-    (k * 2 <= v hl ==> smaller h tl tree depth heap'.[k] heap'.[k * 2]) /\
-    (k * 2 + 1 <= v hl ==> smaller h tl tree depth heap'.[k] heap'.[k * 2 + 1])))
+  let hl = v hl in
+  let heap_elem = heap_elem tl depth in
+  let heap = B.as_seq h heap in
+  let tree = B.as_seq h tree in
+  let depth = B.as_seq h depth in
+  let smaller = cmp tl tree depth in
+  (forall a. a `smaller` a) /\
+  (forall a b. a `smaller` b /\ b `smaller` a ==> a == b) /\
+  (forall a b c. a `smaller` b /\ b `smaller` c ==> a `smaller` c) /\
+  (forall a b. a `smaller` b \/ b `smaller` a) /\
+  (forall (j: pos). j <= hl ==> v heap.[j] < tl) /\
+  (forall (k: nat). (v i <= k /\ k <= hl) ==> (
+    heap_elem heap.[k] /\
+    (k * 2 <= hl ==>
+      heap_elem heap.[k * 2] /\ heap.[k] `smaller` heap.[k * 2]) /\
+    (k * 2 + 1 <= hl ==>
+      heap_elem heap.[k * 2 + 1] /\ heap.[k] `smaller` heap.[k * 2 + 1])))
 
 let well_formed
-  (h: HS.mem) (heap: tree_heap_t) (hl: heap_len_t)
-  (tl: nat) (tree: B.lbuffer ct_data tl) (depth: tree_depth_t) =
-  U32.v hl > 1 ==> partial_well_formed h heap hl tl tree depth 1ul
+  (cmp: cmp_spec) (h: HS.mem)
+  (heap: tree_heap_t) (hl: heap_len_t)
+  (tl: tree_len_t) (tree: B.lbuffer ct_data tl) (depth: tree_depth_t) =
+  partial_well_formed cmp h heap hl tl tree depth 1ul
 
 unfold let permutation_partial (h1 h2: seq U32.t) (root hole: U32.t) =
   let root = U32.v root in let hole = U32.v hole in
@@ -55,3 +76,75 @@ unfold let permutation_partial (h1 h2: seq U32.t) (root hole: U32.t) =
     (h2.[hole] == h1.[root] ==> count h1.[root] h2 == count h1.[root] h1) /\
     (forall (x: U32.t). {:pattern (count x h1) \/ (count x h2)}
       (x <> h1.[root] /\ x <> h2.[hole]) ==> count x h1 == count x h2))
+
+private let rec log2 (a: pos): Tot (n: nat{
+  pow2 n <= a /\ a < pow2 (n + 1)
+}) = if a = 1 then 0 else 1 + log2 (a / 2)
+
+private let rec log2_pow2_lt (a: pos) (n: nat): Lemma
+  (requires n < log2 a)
+  (ensures pow2 n < a) =
+  match n with
+  | 0 -> ()
+  | _ -> log2_pow2_lt (a / 2) (n - 1)
+
+private let rec log2_pow2_gt (a: pos) (n: pos): Lemma
+  (requires a < pow2 n)
+  (ensures log2 a < n) =
+  match (a, n) with
+  | (1, _) | (_, 1) -> ()
+  | _ -> log2_pow2_gt (a / 2) (n - 1)
+
+private let rec parent (a: pos) (i: pos{i <= log2 a}): Tot (res: pos{res < a}) =
+  if i > 1 then parent (a / 2) (i - 1) else a / 2
+
+private let rec parent_next (a: pos) (i: pos{1 < i /\ i <= log2 a}): Lemma
+  (ensures parent a i == parent a (i - 1) / 2) =
+  match i with
+  | 2 -> ()
+  | _ -> parent_next (a / 2) (i - 1)
+
+#set-options "--z3refresh --z3rlimit 512 --fuel 1 --ifuel 0"
+private let rec partial_well_formed_max
+  (cmp: cmp_spec) (h: HS.mem)
+  (heap: tree_heap_t) (hl: heap_len_t)
+  (tl: tree_len_t) (tree: B.lbuffer ct_data tl) (depth: tree_depth_t)
+  (i: nat) (j: pos) : Lemma
+  (requires
+    i < log2 j /\ j <= U32.v hl /\ pow2 i < j /\
+    partial_well_formed cmp h heap hl tl tree depth (U32.uint_to_t (pow2 i)))
+  (ensures
+    pow2 i <= parent j ((log2 j) - i) /\
+    parent j ((log2 j) - i) < pow2 (i + 1) /\
+    cmp tl (B.as_seq h tree) (B.as_seq h depth)
+      (B.as_seq h heap).[parent j ((log2 j) - i)] (B.as_seq h heap).[j])
+  (decreases U32.v hl - pow2 i) =
+  if j < pow2 (i + 2) then begin
+    log2_pow2_lt j i;
+    log2_pow2_gt j (i + 2)
+  end else begin
+    partial_well_formed_max cmp h heap hl tl tree depth (i + 1) j;
+    parent_next j ((log2 j) - i)
+  end
+
+private let heap_max'
+  (cmp: cmp_spec) (h: HS.mem)
+  (heap: tree_heap_t) (hl: heap_len_t)
+  (tl: tree_len_t) (tree: B.lbuffer ct_data tl) (depth: tree_depth_t)
+  (i: pos{1 < i /\ i <= U32.v hl}) : Lemma
+  (requires well_formed cmp h heap hl tl tree depth)
+  (ensures cmp tl (B.as_seq h tree) (B.as_seq h depth)
+    (B.as_seq h heap).[1] (B.as_seq h heap).[i]) =
+  partial_well_formed_max cmp h heap hl tl tree depth 0 i
+
+let heap_max
+  (cmp: cmp_spec) (h: HS.mem)
+  (heap: tree_heap_t) (hl: heap_len_t)
+  (tl: tree_len_t) (tree: B.lbuffer ct_data tl) (depth: tree_depth_t): Lemma
+  (requires well_formed cmp h heap hl tl tree depth)
+  (ensures forall i.
+    let tree = B.as_seq h tree in
+    let depth = B.as_seq h depth in
+    let heap = B.as_seq h heap in
+    1 < i /\ i < U32.v hl ==> cmp tl tree depth heap.[1] heap.[i]) =
+  Classical.forall_intro (Classical.move_requires (heap_max' cmp h heap hl tl tree depth))
